Reworked CSE for operations.
Reworked CSE to also work if the result after the transformation is more
defined than the original value. This allows simplifying comparisons
operations as well as selection operations.
Bug 34849

powerpc/CombineOp.v
@@ -141,18 +141,25 @@ Function combine_op (op: operation) (args: list valnum) : option(operation * lis
       | _ => None
       end
   | Ocmp cond, _ =>
-      match combine_cond cond args with
-      | Some(cond', args') => Some(Ocmp cond', args')
-      | None => None
+      match combine_cond' cond args with
+      | Some b => Some ((if b then Ointconst Int.one else Ointconst Int.zero), nil)
+      | None =>
+          match combine_cond cond args with
+          | Some(cond', args') => Some(Ocmp cond', args')
+          | None => None
+          end
       end
   | Osel cond ty, x :: y :: args =>
-      match combine_cond cond args with
-      | Some (cond', args') => Some (Osel cond' ty, x :: y :: args')
-      | None => None
+      match combine_cond' cond args with
+      | Some b => Some (Omove, (if b then x else y) :: nil)
+      | None =>
+          if eq_valnum x y then Some (Omove, x :: nil) else
+          match combine_cond cond args with
+          | Some (cond', args') => Some (Osel cond' ty, x :: y :: args')
+          | None => None
+          end
       end
   | _, _ => None
   end.
 
 End COMBINE.
-
-
