aarch64/CombineOpproof.v
@@ -204,41 +204,60 @@ Proof.
 Qed.
 
 Theorem combine_op_sound:
-  forall op args op' args',
+  forall op args op' args' r,
   combine_op get op args = Some(op', args') ->
-  eval_operation ge sp op' (map valu args') m = eval_operation ge sp op (map valu args) m.
+  eval_operation ge sp op (map valu args) m = Some r ->
+  exists r', eval_operation ge sp op' (map valu args') m = Some r' /\ Val.lessdef r r'.
 Proof.
   intros. functional inversion H; subst.
   (* addimm - addimm *)
-  - UseGetSound. FuncInv. simpl.
-    rewrite <- H0. rewrite Val.add_assoc. auto.
+  - UseGetSound. exists r; split; auto.
+    rewrite <- H0. simpl. rewrite <- H1. rewrite Val.add_assoc. auto.
   (* andimm - andimm *)
   - UseGetSound; simpl.
-    generalize (Int.eq_spec p m0); rewrite H7; intros.
-    rewrite <- H0. rewrite Val.and_assoc. simpl. fold p. rewrite H1. auto.
-  - UseGetSound; simpl.
-    rewrite <- H0. rewrite Val.and_assoc. auto.
+    generalize (Int.eq_spec p m0); rewrite H8; intros. exists r; split; auto.
+    rewrite <- H0. simpl. rewrite <- H1. rewrite Val.and_assoc.
+    simpl. fold p. rewrite H2. auto.
+  - UseGetSound; simpl. exists r; split; auto.
+    rewrite <- H0. simpl. rewrite <- H1. rewrite Val.and_assoc. auto.
   (* orimm - orimm *)
-  - UseGetSound. simpl. rewrite <- H0. rewrite Val.or_assoc. auto.
+  - UseGetSound. exists r; split; auto. rewrite <- H0. simpl. rewrite <- H1. rewrite Val.or_assoc. auto.
   (* xorimm - xorimm *)
-  - UseGetSound. simpl. rewrite <- H0. rewrite Val.xor_assoc. auto.
+  - UseGetSound. exists r; split; auto. rewrite <- H0. simpl. rewrite <- H1. rewrite Val.xor_assoc. auto.
   (* addlimm - addlimm *)
-  - UseGetSound. FuncInv. simpl.
-    rewrite <- H0. rewrite Val.addl_assoc. auto.
+  - UseGetSound. exists r; split; auto.
+    rewrite <- H0. simpl. rewrite <- H1. rewrite Val.addl_assoc. auto.
   (* andlimm - andlimm *)
-  - UseGetSound; simpl.
-    generalize (Int64.eq_spec p m0); rewrite H7; intros.
-    rewrite <- H0. rewrite Val.andl_assoc. simpl. fold p. rewrite H1. auto.
-  - UseGetSound; simpl.
-    rewrite <- H0. rewrite Val.andl_assoc. auto.
+  - UseGetSound. exists r; split; auto.
+    generalize (Int64.eq_spec p m0); rewrite H8; intros.
+    rewrite <- H0. simpl. rewrite <- H1. rewrite Val.andl_assoc. simpl. fold p. rewrite H2. auto.
+  - UseGetSound. exists r; split; auto.
+    rewrite <- H0. simpl. rewrite <- H1. rewrite Val.andl_assoc. auto.
   (* orlimm - orlimm *)
-  - UseGetSound. simpl. rewrite <- H0. rewrite Val.orl_assoc. auto.
+  - UseGetSound. exists r; split; auto. rewrite <- H0. simpl. rewrite <- H1. rewrite Val.orl_assoc. auto.
   (* xorlimm - xorlimm *)
-  - UseGetSound. simpl. rewrite <- H0. rewrite Val.xorl_assoc. auto.
-  (* cmp *)
-  - simpl. decEq; decEq. eapply combine_cond_sound; eauto.
-  (* sel *)
-  - simpl. erewrite combine_cond_sound; eauto.
+  - UseGetSound. exists r; split; auto. rewrite <- H0. simpl. rewrite <- H1. rewrite Val.xorl_assoc. auto.
+  (* cmp true *)
+  - exists Vtrue; split; auto. inv H0. destruct (eval_condition cond (map valu args) m) eqn:?; auto.
+    rewrite (combine_cond'_sound cond args b true); eauto.
+  (* cmp false *)
+  - exists Vfalse; split; auto. inv H0. destruct (eval_condition cond (map valu args) m) eqn:?; auto.
+    rewrite (combine_cond'_sound cond args b false); eauto.
+  (* cmp reduce *)
+  - exists r; split; auto. decEq; decEq. simpl. erewrite combine_cond_sound; eauto.
+  (* sel cond true *)
+  - exists (valu x). simpl in H0.
+   destruct (eval_condition cond (map valu args1) m) eqn:?; simpl; split; auto; inv H0; auto.
+   rewrite (combine_cond'_sound cond args1 b true); eauto.  destruct (valu x), ty; auto.
+  (* sel cond false *)
+  - exists (valu y). simpl in H0.
+   destruct (eval_condition cond (map valu args1) m) eqn:?; simpl; split; auto; inv H0; auto.
+   rewrite (combine_cond'_sound cond args1 b false); eauto.  destruct (valu y), ty; auto.
+  (* sel cond same *)
+  - exists (valu y); split; auto. inv H0. destruct (eval_condition cond (map valu args1) m); auto.
+   simpl. destruct b, (valu y), ty; auto.
+  - exists r; split; auto. rewrite <- H0.
+   simpl. erewrite combine_cond_sound; eauto.
 Qed.
 
 End COMBINE.
