x86/CombineOpproof.v
@@ -189,31 +189,49 @@ Proof.
 Qed.
 
 Theorem combine_op_sound:
-  forall op args op' args',
+  forall op args op' args' r,
   combine_op get op args = Some(op', args') ->
-  eval_operation ge sp op' (map valu args') m = eval_operation ge sp op (map valu args) m.
+  eval_operation ge sp op (map valu args) m = Some r ->
+  exists r', eval_operation ge sp op' (map valu args') m = Some r' /\ Val.lessdef r r'.
 Proof.
   intros. functional inversion H; subst.
 (* lea-lea *)
-  simpl. eapply combine_addr_32_sound; eauto.
+ - exists r; split; auto. rewrite <- H0. eapply combine_addr_32_sound; eauto.
 (* leal-leal *)
-  simpl. eapply combine_addr_64_sound; eauto.
+ - exists r; split; auto.  rewrite <- H0. eapply combine_addr_64_sound; eauto.
 (* andimm - andimm *)
-  UseGetSound; simpl. rewrite <- H0. rewrite Val.and_assoc. auto.
+ - UseGetSound. exists r; split; auto. rewrite <- H0. simpl. rewrite <- H1. rewrite Val.and_assoc. auto.
 (* orimm - orimm *)
-  UseGetSound; simpl. rewrite <- H0. rewrite Val.or_assoc. auto.
+ - UseGetSound. exists r; split; auto. rewrite <- H0. simpl. rewrite <- H1. rewrite Val.or_assoc. auto.
 (* xorimm - xorimm *)
-  UseGetSound; simpl. rewrite <- H0. rewrite Val.xor_assoc. auto.
+ - UseGetSound. exists r; split; auto. rewrite <- H0. simpl. rewrite <- H1. rewrite Val.xor_assoc. auto.
 (* andimm - andimm *)
-  UseGetSound; simpl. rewrite <- H0. rewrite Val.andl_assoc. auto.
+ - UseGetSound. exists r; split; auto. rewrite <- H0. simpl. rewrite <- H1. rewrite Val.andl_assoc. auto.
 (* orimm - orimm *)
-  UseGetSound; simpl. rewrite <- H0. rewrite Val.orl_assoc. auto.
+ - UseGetSound. exists r; split; auto. rewrite <- H0. simpl. rewrite <- H1. rewrite Val.orl_assoc. auto.
 (* xorimm - xorimm *)
-  UseGetSound; simpl. rewrite <- H0. rewrite Val.xorl_assoc. auto.
-(* cmp *)
-  simpl. decEq; decEq. eapply combine_cond_sound; eauto.
-(* sel *)
-  simpl. erewrite combine_cond_sound; eauto.
+ - UseGetSound. exists r; split; auto. rewrite <- H0. simpl. rewrite <- H1. rewrite Val.xorl_assoc. auto.
+ (* cmp true *)
+ - exists Vtrue; split; auto. inv H0. destruct (eval_condition cond (map valu args) m) eqn:?; auto.
+   rewrite (combine_cond'_sound cond args b true); eauto.
+ (* cmp false *)
+ - exists Vfalse; split; auto. inv H0. destruct (eval_condition cond (map valu args) m) eqn:?; auto.
+   rewrite (combine_cond'_sound cond args b false); eauto.
+ (* cmp reduce *)
+ - exists r; split; auto. decEq; decEq. simpl. erewrite combine_cond_sound; eauto.
+ (* sel cond true *)
+ - exists (valu x). simpl in H0.
+   destruct (eval_condition cond (map valu args1) m) eqn:?; simpl; split; auto; inv H0; auto.
+   rewrite (combine_cond'_sound cond args1 b true); eauto.  destruct (valu x), ty; auto.
+ (* sel cond false *)
+ - exists (valu y). simpl in H0.
+   destruct (eval_condition cond (map valu args1) m) eqn:?; simpl; split; auto; inv H0; auto.
+   rewrite (combine_cond'_sound cond args1 b false); eauto.  destruct (valu y), ty; auto.
+ (* sel cond same *)
+ - exists (valu y); split; auto. inv H0. destruct (eval_condition cond (map valu args1) m); auto.
+   simpl. destruct b, (valu y), ty; auto.
+ - exists r; split; auto. rewrite <- H0.
+   simpl. erewrite combine_cond_sound; eauto.
 Qed.
 
 End COMBINE.
